finish exercixe 1 from class 5

aulas/aula5.dfy
@@ -2,43 +2,94 @@ type T = int // for demo purposes, but could be another type
  
 class {:autocontracts} Deque {
     // (Private) concrete state variables 
-    const list: array<T>; // circular array, from list[start] (front) to 
-                             list[(start+size-1) % list.Length] (back) 
+    const list: array<T>; // circular array, from list[start] (front) to  list[(start+size-1) % list.Length] (back) 
     var start : nat; 
     var size : nat;
+
+    // (Public) ghost variables used for specification purposes only
+    // and so, they do not go to the executable file
+    ghost var elems: seq<T>;  // front at head, back at tail
+    ghost const capacity: nat; 
+
+    predicate Valid() {
+        // consistency of concrete states variables
+        (size <= list.Length) &&
+        (/*size > 0 ==>*/ 0 <= start < list.Length) && // if size > 0 then we need to verify that 0 <= start < list.Length
+        // consistency between concrete and abstract states variables
+        (capacity == list.Length) &&
+        (elems == if start + size <= list.Length // nao da a volta
+                    then list[start..start+size]
+                    else list[start..] + list[..start + size - list.Length])
+        // OR
+        /*
+        && |elems| == size &&
+        forall i :: 0 <= i < size ==> list[(start + i) % list.Length] == elems[i]
+        */
+        
+    }
  
-    constructor (capacity: nat) {
+    constructor (capacity: nat)
+        requires capacity > 0
+        ensures elems == [] && this.capacity == capacity
+    {
+        // update concrete variables
         list := new T[capacity];
         start := 0;
         size := 0;
+        // update abstract variables
+        this.capacity := capacity;
+        elems := [];
     }
  
-    predicate method isEmpty() {
+    predicate method isEmpty()
+        ensures isEmpty() <==> elems == []
+    {
         size == 0
     }
     
-    predicate method isFull() {
+    predicate method isFull()
+        ensures isFull() <==> |elems| == capacity
+    {
         size == list.Length
     }
  
-    function method front() : T {
+    function method front() : T 
+        requires !isEmpty()
+        ensures front() == elems[0]
+    {
         list[start]
     }
  
-    function method back() : T {
+    function method back() : T
+        requires !isEmpty()
+        ensures back() == elems[|elems| - 1]
+    {
         list[(start + size - 1) % list.Length] 
     }
     
-    method push_back(x : T) {
+    method push_back(x : T)
+        requires !isFull()
+        ensures elems == old(elems) + [x]
+    {
         list[(start + size) % list.Length] := x;
         size := size + 1;
+        // updating abstract variables
+        elems := elems + [x];
     }
  
-    method pop_back() {
+    method pop_back()
+        requires !isEmpty()
+        ensures elems == old(elems[..|elems| - 1])
+    {
         size := size - 1;
+        // updating abstract variables
+        elems := elems[..|elems| - 1];
     }
  
-    method push_front(x : T) {
+    method push_front(x : T)
+        requires !isFull()
+        ensures elems == [x] + old(elems)
+    {
         if start > 0 {
             start := start - 1;
         }
@@ -47,9 +98,14 @@ class {:autocontracts} Deque {
         }
         list[start] := x;
         size := size + 1;
+        // updating abstract variables
+        elems := [x] + elems;
     }    
  
-    method pop_front() {
+    method pop_front()
+        requires !isEmpty()
+        ensures elems == old(elems[1..])
+    {
         if start + 1 < list.Length {
             start := start + 1;
         }
@@ -57,6 +113,8 @@ class {:autocontracts} Deque {
             start := 0;
         }
         size := size - 1;
+        // updating abstract variables
+        elems := elems[1..];
     } 
 }
  
